clean up proofs + make storage requirements precise

Diff_Arr_Safe.thy
@@ -10,14 +10,10 @@ qualified definition lookup where
     len \<leftarrow>  Diff_Arr.length arr;
     if i < len
     then Diff_Arr.lookup arr i
-    else do { 
-      arr \<leftarrow> Diff_Arr.realize arr;
-      xs  \<leftarrow> Array.freeze arr;
-      return (xs ! i)
-    }
+    else return (undefined(i - len))
   }"
 
-qualified definition update  where
+qualified definition update where
   "update arr i v = do {
     len \<leftarrow> Diff_Arr.length arr;
     if i < len
@@ -32,28 +28,25 @@ lemma update_safe [sep_heap_rules]: "
      Diff_Arr_Safe.update diff_arr i v
   <\<lambda>diff_arr. \<exists>\<^sub>At'. master_assn t' * 
     \<up>((\<forall>xs' diff_arr'. t \<turnstile> xs' \<sim> diff_arr' \<longrightarrow> t' \<turnstile> xs' \<sim> diff_arr') 
-      \<and> (t' \<turnstile> xs[i := v] \<sim> diff_arr))>\<^sub>t"
+      \<and> (t' \<turnstile> xs[i := v] \<sim> diff_arr))>"
   unfolding Diff_Arr_Safe.update_def
   apply sep_auto
-  apply(rule fi_rule[OF length])
-  apply sep_auto
-  apply sep_auto
+  apply(rule fi_rule[OF length, where F = emp])
+  apply sep_auto+
   apply(rule cons_post_rule)
-  apply(rule fi_rule[OF update])
+  apply(rule fi_rule[OF update, where F = emp])
   by sep_auto+
 
 lemma lookup_safe [sep_heap_rules]: "
   <master_assn t * \<up>(t \<turnstile> xs \<sim> a)> 
      Diff_Arr_Safe.lookup a i 
-  <\<lambda>r. master_assn t * \<up>(r = xs!i)>\<^sub>t"
-  unfolding  Diff_Arr_Safe.lookup_def
+  <\<lambda>r. master_assn t * \<up>(r = xs!i)>"
+  unfolding Diff_Arr_Safe.lookup_def
   apply sep_auto
-  apply(rule fi_rule[OF length])
-  apply sep_auto+
-  apply(rule cons_post_rule)
-  apply(rule fi_rule[OF lookup])
-  apply sep_auto+
-  apply(rule fi_rule[OF realize])
-  by sep_auto+
+  using length 
+  apply sep_auto
+  apply sep_auto
+  using lookup
+  by(sep_auto simp: nth_undefined[of xs i])+
 
 end
