Diff_Arr.thy
@@ -96,82 +96,65 @@ next
     by sep_auto
 qed 
 
-lemma from_array [sep_heap_rules]:
-    "<a \<mapsto>\<^sub>a xs> Diff_Arr.from_array a <\<lambda>r. \<exists>\<^sub>At. master_assn t * \<up>(t \<turnstile> xs \<sim> r)>"
-  unfolding Diff_Arr.from_array_def master_assn_def diff_arr_rel_def
-  apply vcg
-  subgoal for r
-    apply(rule ent_ex_postI[where x = "[(r, Array' xs)]"])
-    apply(subst exI[where x = "0"])
-    by(sep_auto simp: ent_ex_postI[where x = "cell.Array a"])+
-  done
-
-lemma from_list [sep_heap_rules]:
-    "<emp> Diff_Arr.from_list xs <\<lambda>r. \<exists>\<^sub>At. master_assn t * \<up>(t \<turnstile> xs \<sim> r)>"
-  unfolding Diff_Arr.from_list_def 
-  by sep_auto
-
+(* TODO: Is it okay to have both from_array'/from_list' and from_array/from_list 
+         in sep_heap_rules? *)
 lemma from_array' [sep_heap_rules]: 
- "<a \<mapsto>\<^sub>a xs * master_assn t>
-     Diff_Arr.from_array a      
-  <\<lambda>r. let t' = (r, Array' xs)#t 
-    in master_assn t' * \<up>(diff_arr_rel t' xs r)>"
-  unfolding Diff_Arr.from_array_def Let_def diff_arr_rel_def
-  by(sep_auto simp: exI[where x = "0"] master_assn_def)
+  "<a \<mapsto>\<^sub>a xs>
+      Diff_Arr.from_array a
+   <\<lambda>r. let t = [(r, Array' xs)] 
+        in master_assn t * \<up>(t \<turnstile> xs \<sim> r)>"
+  unfolding Diff_Arr.from_array_def diff_arr_rel_def master_assn_def
+  apply auto
+  by(sep_auto simp: exI[where x = "0"])
  
 lemma from_list' [sep_heap_rules]:
-    "<master_assn t> 
-      Diff_Arr.from_list xs 
-     <\<lambda>r. let t' = (r, Array' xs) # t 
-          in  master_assn t' * \<up>(t' \<turnstile> xs \<sim> r)>"
+  "<emp> 
+    Diff_Arr.from_list xs 
+   <\<lambda>r. let t = [(r, Array' xs)]
+        in  master_assn t * \<up>(t \<turnstile> xs \<sim> r)>"
   unfolding Diff_Arr.from_list_def
   by sep_auto
+
+lemma from_array [sep_heap_rules]:
+  "<a \<mapsto>\<^sub>a xs> Diff_Arr.from_array a <\<lambda>r. \<exists>\<^sub>At. master_assn t * \<up>(t \<turnstile> xs \<sim> r)>"
+  by(sep_auto simp: Let_def)
+
+lemma from_list [sep_heap_rules]:
+  "<emp> Diff_Arr.from_list xs <\<lambda>r. \<exists>\<^sub>At. master_assn t * \<up>(t \<turnstile> xs \<sim> r)>"
+  by(sep_auto simp: Let_def)
 
 lemma lookup_aux: "
   <\<up>(t \<turnstile> xs \<sim>\<^sub>n a \<and> i < length xs) * master_assn t >
       Diff_Arr.lookup a i 
-  <\<lambda>r. master_assn t * \<up>(r = xs!i)>\<^sub>t"
+  <\<lambda>r. master_assn t * \<up>(r = xs!i)>"
 proof(induction n arbitrary: xs a)
   case 0
-  show ?case
-    apply(sep_auto)
+  then show ?case 
+    apply sep_auto
     apply(subst lookup.simps)
     apply(sep_drule r: open_master_assn)
-    apply(sep_auto)
-    apply(sep_drule r: close_master_assn_array)
-    by sep_auto
+    by(sep_auto simp: close_master_assn_array)
 next
   case (Suc n)
-
-  show ?case
+  then show ?case
     apply(sep_auto)
     apply(subst lookup.simps)
     apply(sep_drule r: open_master_assn)
-    apply sep_auto
-    apply (sep_drule r: close_master_assn_upd)
-    apply sep_auto
-    apply (sep_drule r: close_master_assn_upd)
-    apply sep_auto
-    apply (rule cons_post_rule)
-    apply (rule fi_rule[OF Suc.IH])
-    by sep_auto+
+    by(sep_auto simp: close_master_assn_upd')
 qed
 
 lemma lookup [sep_heap_rules]: "
   <master_assn t * \<up>(t \<turnstile> xs \<sim> a \<and> i < length xs)> 
      Diff_Arr.lookup a i 
-  <\<lambda>r. master_assn t * \<up>(r = xs!i)>\<^sub>t
-" unfolding diff_arr_rel_def
-  apply(sep_auto)
-  apply(rule cons_post_rule)
-  apply(rule fi_rule[OF lookup_aux])
-  by solve_entails
+  <\<lambda>r. master_assn t * \<up>(r = xs!i)>"
+  unfolding diff_arr_rel_def
+  using lookup_aux[of t]
+  by sep_auto
 
-lemma realize_aux: "
-  <master_assn t * \<up>(t \<turnstile> xs \<sim>\<^sub>n diff_arr)> 
+lemma realize_aux: 
+ "<master_assn t * \<up>(t \<turnstile> xs \<sim>\<^sub>n diff_arr)> 
      Diff_Arr.realize diff_arr
-  <\<lambda>arr. master_assn t * \<up>(t \<turnstile> xs \<sim>\<^sub>n diff_arr) * arr \<mapsto>\<^sub>a xs>
-" 
+  <\<lambda>arr. master_assn t * arr \<mapsto>\<^sub>a xs>" 
 proof(induction n arbitrary: t diff_arr xs)
   case 0
   then show ?case
@@ -189,148 +172,149 @@ next
     apply(sep_drule r: open_master_assn)
     apply sep_auto
     apply(sep_drule r: close_master_assn_upd)
-    apply sep_auto
+    apply(sep_auto)
     apply(sep_drule r: open_master_assn)
     apply sep_auto
     apply(sep_drule r: close_master_assn_upd)
     by sep_auto
 qed
 
-lemma realize [sep_heap_rules]: "
-   <master_assn t * \<up>(t \<turnstile> xs \<sim> diff_arr)> 
+lemma realize [sep_heap_rules]: 
+  "<master_assn t * \<up>(t \<turnstile> xs \<sim> diff_arr)> 
      Diff_Arr.realize diff_arr
-  <\<lambda>arr. master_assn t * \<up>(t \<turnstile> xs \<sim> diff_arr) * arr \<mapsto>\<^sub>a xs>
-" 
+   <\<lambda>arr. master_assn t * arr \<mapsto>\<^sub>a xs>" 
   unfolding diff_arr_rel_def
-  apply sep_auto
-  subgoal for n
-    using realize_aux[of t xs n diff_arr]
-    by sep_auto
-  done
+  using realize_aux[of t]
+  by sep_auto
 
-(* TODO: Simplify *)
-lemma update[sep_heap_rules]: "
-  <master_assn t * \<up>(t \<turnstile> xs \<sim> diff_arr \<and> i < length xs)> 
-     Diff_Arr.update diff_arr i v
-  <\<lambda>diff_arr. \<exists>\<^sub>At'. master_assn t' * 
-    \<up>((\<forall>xs' diff_arr'. t \<turnstile> xs' \<sim> diff_arr' \<longrightarrow> t' \<turnstile> xs' \<sim> diff_arr') \<and> 
-      (t' \<turnstile> xs[i := v] \<sim> diff_arr))>\<^sub>t"
-  apply(subst update.simps)
-  unfolding diff_arr_rel_def
-  apply auto
-  subgoal for n
-  proof(induction "n = 0")
+lemma update_diff_arr_rel: "\<lbrakk>
+  i < length xs; 
+  (diff_arr, Array' xs) \<in>\<^sub>L t; 
+  distinct (map fst t);
+  t \<turnstile> xs' \<sim>\<^sub>n' diff_arr'
+\<rbrakk> \<Longrightarrow> \<exists>n. (new_diff_arr, Array' (xs[i := v])) #
+          (diff_arr, Upd' i (xs ! i) new_diff_arr) #
+          remove1 (diff_arr, Array' xs) t \<turnstile> xs' \<sim>\<^sub>n diff_arr'"
+proof(induction t==t xs' n' diff_arr' arbitrary: xs' diff_arr' rule: diff_arr_rel'.induct)
+  case (1 xs' diff_arr')
+  then show ?case 
+  proof(cases "diff_arr' = diff_arr")
     case True
-    then show ?thesis 
+  
+    with 1 have "distinct (map fst t)" 
+      by auto
+  
+    with 1 True have "xs' = xs"
+      using distinct_map_fstD[of t]
+      by auto
+  
+    with True 1 show ?thesis
       apply -
-      apply(rule hoare_triple_preI)
-      apply(drule master_assn_distinct)
-      apply simp
-      apply(sep_drule r: open_master_assn)
-      apply(sep_auto eintros del: exI)
-      subgoal for new_arr new_diff_arr
-        apply(rule exI[where x = "
-                      (new_diff_arr, Array' (xs[i := v]))
-                   #  (diff_arr, Upd' i (xs ! i) new_diff_arr)
-                   #  (remove1 (diff_arr, Array' xs) t)"
-                ]) 
-        apply sep_auto
-        subgoal for xs' diff_arr' h n' as
-        proof(induction t==t xs' n' diff_arr' arbitrary: xs' diff_arr' rule: diff_arr_rel'.induct)
-          case (1 xs' diff_arr')
-          then show ?case 
-          proof(cases "diff_arr' = diff_arr")
-            case True
-
-            with 1 have "distinct (map fst t)" 
-              by auto
-
-            with 1 True have "xs' = xs"
-              by (meson cell'.inject(1) distinct_map_fstD diff_arr_rel'.simps(1))
-
-            with True 1 show ?thesis
-              apply -
-              apply(rule exI[where x = 1])
-              apply sep_auto
-              apply(rule exI[where x = i])
-              apply(rule exI[where x = "xs ! i"])
-              apply(rule exI[where x = new_diff_arr])
-              by sep_auto
-          next
-            case False
-            with 1 show ?thesis
-              apply -
-              apply(rule exI[where x = 0])
-              by sep_auto
-          qed
-        next
-          case (2 xs' n' diff_arr')
-          note LA_REL_PREM = \<open>diff_arr_rel' t  xs' (Suc n') diff_arr'\<close>
-          note OTHER_PREMS = 2(2) 2(3) 2(4) 2(5) 2(7)
-
-          from LA_REL_PREM show ?case
-            apply sep_auto
-            subgoal for i v diff_arr'' xs''
-              using "2.hyps"[of xs'' diff_arr''] OTHER_PREMS
-              apply(sep_auto)
-              subgoal for n''
-                apply(rule exI[where x = "Suc n''"])
-                by(sep_auto)
-              done
-            done
-        qed
-        apply (meson diff_arr_rel'.simps(1) list.set_intros(1))
-        by(sep_auto simp: open_master_assn_cons)
-      done
+      apply(rule exI[where x = 1])
+      apply(sep_auto)
+      apply(rule exI[where x = i])
+      apply(rule exI[where x = "xs ! i"])
+      apply(rule exI[where x = new_diff_arr])
+      by sep_auto
   next
     case False
-    then show ?thesis 
-      apply(sep_auto heap: ref_lookup_upd)
-      apply(rule fi_rule[OF realize_aux])
-      apply(sep_auto eintros del: exI)+
-      subgoal for new_arr new_diff_arr
-        apply(cases "(new_diff_arr, Array' (xs[i := v])) \<in>\<^sub>L t")
-        
-        subgoal
-          apply-
-          apply(rule exI[where x = "t"])
-          by(sep_auto intro: exI[where x = 0])
-        
-        subgoal
-          apply-
-          apply(rule exI[where x = "(new_diff_arr, Array' (xs[i := v])) #  t"])
-          apply sep_auto
-          using diff_arr_rel'_cons apply blast
-          by(sep_auto simp: open_master_assn_cons intro: exI[where x = 0])+
-        
-        done
-      done
+    with 1 show ?thesis
+      by(sep_auto simp: exI[where x = 0])
   qed
-  done
+next
+  case (2 xs' n' diff_arr')
+
+  then obtain i' v' diff_arr'' xs'' where unfold_diff_arr_rel:
+      "(diff_arr', Upd' i' v' diff_arr'') \<in>\<^sub>L t" 
+      "t \<turnstile> xs'' \<sim>\<^sub>n' diff_arr''" 
+      "i' < length xs''"
+      "xs' = xs''[i' := v']"
+    by sep_auto
+
+  with 2 obtain n'' where 
+     "(new_diff_arr, Array' (xs[i := v])) #
+      (diff_arr, Upd' i (xs ! i) new_diff_arr) #
+      remove1 (diff_arr, Array' xs) t \<turnstile> xs'' \<sim>\<^sub>n'' diff_arr''"
+    by sep_auto
+
+  with unfold_diff_arr_rel show ?case
+    apply sep_auto
+    apply(rule exI[where x = "Suc n''"])
+    by sep_auto
+qed
+
+lemma update_aux: 
+  assumes
+    "i < length xs"
+    "t \<turnstile> xs \<sim>\<^sub>n diff_arr"
+  shows
+    "<master_assn t> 
+       Diff_Arr.update diff_arr i v
+     <\<lambda>diff_arr. \<exists>\<^sub>At'. master_assn t' * 
+       \<up>((\<forall>xs' diff_arr'. t \<turnstile> xs' \<sim> diff_arr' \<longrightarrow> t' \<turnstile> xs' \<sim> diff_arr') \<and> 
+         (t' \<turnstile> xs[i := v] \<sim> diff_arr))>"
+proof(cases "n = 0")
+  case True
+  with assms show ?thesis
+      unfolding diff_arr_rel_def
+      apply(simp add: update.simps)
+      apply(hoare_triple_preI rule: master_assn_distinct)
+      apply(sep_drule r: open_master_assn)
+      apply(sep_auto eintros del: exI)       
+      subgoal for new_arr new_diff_arr
+        apply(rule exI[where x = 
+                     "(new_diff_arr, Array' (xs[i := v])) #
+                      (diff_arr, Upd' i (xs ! i) new_diff_arr) #
+                      (remove1 (diff_arr, Array' xs) t)"
+                ]) 
+        by(sep_auto simp: update_diff_arr_rel open_master_assn_cons exI[where x = 0])
+      done
+next
+  case False
+
+  with realize_aux assms show ?thesis
+  unfolding diff_arr_rel_def
+  apply(subst update.simps)
+  apply(sep_auto heap: ref_lookup_upd eintros del: exI)
+  subgoal for new_arr new_diff_arr
+    apply(rule exI[where x = "(new_diff_arr, Array' (xs[i := v])) #  t"])
+    by(sep_auto simp: diff_arr_rel'_cons' exI[where x = 0] open_master_assn_cons[of new_diff_arr])
+   done
+qed
+
+lemma update[sep_heap_rules]: 
+  "<master_assn t * \<up>(t \<turnstile> xs \<sim> diff_arr \<and> i < length xs)> 
+     Diff_Arr.update diff_arr i v
+   <\<lambda>diff_arr. \<exists>\<^sub>At'. master_assn t' * 
+    \<up>((\<forall>xs' diff_arr'. t \<turnstile> xs' \<sim> diff_arr' \<longrightarrow> t' \<turnstile> xs' \<sim> diff_arr') \<and> 
+      (t' \<turnstile> xs[i := v] \<sim> diff_arr))>"
+  by(sep_auto heap: update_aux simp: diff_arr_rel_def)
+
+lemma length_aux: "t \<turnstile> xs \<sim>\<^sub>n diff_arr \<Longrightarrow> 
+  <master_assn t> 
+    Diff_Arr.length diff_arr 
+  <\<lambda>len. master_assn t * \<up>(len = length xs)>"
+proof(induction t xs n diff_arr rule: diff_arr_rel'.induct)
+  case 1
+  then show ?case 
+    apply sep_auto
+    apply(subst length.simps)
+    apply(sep_drule r: open_master_assn)
+    by(sep_auto simp: close_master_assn_array)
+next
+  case 2
+  then show ?case 
+    apply sep_auto
+    apply(subst length.simps)
+    apply(sep_drule r: open_master_assn)
+    by(sep_auto simp: close_master_assn_upd')
+qed
 
 lemma length[sep_heap_rules]: "
   <master_assn t * \<up>(t \<turnstile> xs \<sim> diff_arr)> 
-    Diff_Arr.length diff_arr 
-  <\<lambda>len. master_assn t * \<up>(t \<turnstile> xs \<sim> diff_arr \<and> len = length xs)>"
-  apply(subst length.simps)
+    Diff_Arr.length diff_arr
+  <\<lambda>len. master_assn t * \<up>(len = length xs)>"
   unfolding diff_arr_rel_def
-  apply auto
-  subgoal for n
-  proof(induction t xs n diff_arr rule: diff_arr_rel'.induct)
-    case (1 t xs a)
-    then show ?case 
-      apply simp
-      apply(sep_drule r: open_master_assn)
-      by(sep_auto simp: close_master_assn_array)
-  next
-    case (2 t xs n a)
-    then show ?case 
-      apply auto
-      apply(sep_drule r: open_master_assn)
-      apply(sep_auto simp: close_master_assn_upd')
-      apply(subst length.simps)
-      by sep_auto
-  qed
-  done
+  by(sep_auto heap: length_aux)
 
 end
